src/FcEtt/ett_inf.v
@@ -1,3 +1,4 @@
+Require Import Coq.Arith.Wf_nat.
 Require Import Coq.Logic.FunctionalExtensionality.
 Require Import Coq.Program.Equality.
 
